Push BALLOCC (BALLOC with cache of free blocks) up the stack. Balloc, BlockPtr, and Inode specs and proofs checkout Some of BFile proofs are broken Need to perculate change in BFile spec further up the stack

src/BFile.v
@@ -33,6 +33,7 @@ Require Import MapUtils.
 Require Import Structures.OrderedType.
 Require Import Structures.OrderedTypeEx.
 Require Import StringUtils.
+Require Import Balloc.
 
 
 Import ListNotations.
@@ -55,15 +56,18 @@ Module BFM := MapMem Nat_as_OT BFcache.
 
 Module BFILE.
 
+
   Record memstate := mk_memstate {
     MSAlloc : bool;         (* which block allocator to use? *)
     MSLL : LOG.memstate;    (* lower-level state *)
+    MSAllocC: (BALLOCC.BmapCacheType * BALLOCC.BmapCacheType); 
     MSCache : BFcache_type
   }.
 
   Ltac msalloc_eq :=
     repeat match goal with
     | [ H: MSAlloc _ = MSAlloc _ |- _ ] => rewrite H in *; clear H
+    | [ H: MSAlloc _ = MSAllocC _ |- _ ] => rewrite H in *; clear H
     | [ H: MSCache _ = MSCache _ |- _ ] => rewrite H in *; clear H
     end.
 
@@ -71,58 +75,58 @@ Module BFILE.
   (* interface implementation *)
 
   Definition getlen lxp ixp inum fms :=
-    let '(al, ms, cache) := (MSAlloc fms, MSLL fms, MSCache fms) in
+    let '(al, ms, alc, cache) := (MSAlloc fms, MSLL fms, MSAllocC fms, MSCache fms) in
     let^ (ms, n) <- INODE.getlen lxp ixp inum ms;
-    Ret ^(mk_memstate al ms cache, n).
+    Ret ^(mk_memstate al ms alc cache, n).
 
   Definition getattrs lxp ixp inum fms :=
-    let '(al, ms, cache) := (MSAlloc fms, MSLL fms, MSCache fms) in
+    let '(al, ms, alc, cache) := (MSAlloc fms, MSLL fms, MSAllocC fms, MSCache fms) in
     let^ (ms, n) <- INODE.getattrs lxp ixp inum ms;
-    Ret ^(mk_memstate al ms cache, n).
+    Ret ^(mk_memstate al ms alc cache, n).
 
   Definition setattrs lxp ixp inum a fms :=
-    let '(al, ms, cache) := (MSAlloc fms, MSLL fms, MSCache fms) in
+    let '(al, ms, alc, cache) := (MSAlloc fms, MSLL fms,  MSAllocC fms, MSCache fms) in
     ms <- INODE.setattrs lxp ixp inum a ms;
-    Ret (mk_memstate al ms cache).
+    Ret (mk_memstate al ms alc cache).
 
   Definition updattr lxp ixp inum kv fms :=
-    let '(al, ms, cache) := (MSAlloc fms, MSLL fms, MSCache fms) in
+    let '(al, ms, alc, cache) := (MSAlloc fms, MSLL fms, MSAllocC fms, MSCache fms) in
     ms <- INODE.updattr lxp ixp inum kv ms;
-    Ret (mk_memstate al ms cache).
+    Ret (mk_memstate al ms alc cache).
 
   Definition read lxp ixp inum off fms :=
-    let '(al, ms, cache) := (MSAlloc fms, MSLL fms, MSCache fms) in
+    let '(al, ms, alc, cache) := (MSAlloc fms, MSLL fms, MSAllocC fms, MSCache fms) in
     let^ (ms, bn) <-INODE.getbnum lxp ixp inum off ms;
     let^ (ms, v) <- LOG.read lxp (# bn) ms;
-    Ret ^(mk_memstate al ms cache, v).
+    Ret ^(mk_memstate al ms alc cache, v).
 
   Definition write lxp ixp inum off v fms :=
-    let '(al, ms, cache) := (MSAlloc fms, MSLL fms, MSCache fms) in
+    let '(al, ms, alc, cache) := (MSAlloc fms, MSLL fms, MSAllocC fms, MSCache fms) in
     let^ (ms, bn) <-INODE.getbnum lxp ixp inum off ms;
     ms <- LOG.write lxp (# bn) v ms;
-    Ret (mk_memstate al ms cache).
+    Ret (mk_memstate al ms alc cache).
 
   Definition dwrite lxp ixp inum off v fms :=
-    let '(al, ms, cache) := (MSAlloc fms, MSLL fms, MSCache fms) in
+    let '(al, ms, alc, cache) := (MSAlloc fms, MSLL fms, MSAllocC fms, MSCache fms) in
     let^ (ms, bn) <- INODE.getbnum lxp ixp inum off ms;
     ms <- LOG.dwrite lxp (# bn) v ms;
-    Ret (mk_memstate al ms cache).
+    Ret (mk_memstate al ms alc cache).
 
   Definition datasync lxp ixp inum fms :=
-    let '(al, ms, cache) := (MSAlloc fms, MSLL fms, MSCache fms) in
+    let '(al, ms, alc, cache) := (MSAlloc fms, MSLL fms, MSAllocC fms, MSCache fms) in
     let^ (ms, bns) <- INODE.getallbnum lxp ixp inum ms;
     ms <- LOG.dsync_vecs lxp (map (@wordToNat _) bns) ms;
-    Ret (mk_memstate al ms cache).
+    Ret (mk_memstate al ms alc cache).
 
   Definition sync lxp (ixp : INODE.IRecSig.xparams) fms :=
-    let '(al, ms, cache) := (MSAlloc fms, MSLL fms, MSCache fms) in
+    let '(al, ms, alc, cache) := (MSAlloc fms, MSLL fms, MSAllocC fms, MSCache fms) in
     ms <- LOG.flushall lxp ms;
-    Ret (mk_memstate (negb al) ms cache).
+    Ret (mk_memstate (negb al) ms alc cache).
 
   Definition sync_noop lxp (ixp : INODE.IRecSig.xparams) fms :=
-    let '(al, ms, cache) := (MSAlloc fms, MSLL fms, MSCache fms) in
+    let '(al, ms, alc, cache) := (MSAlloc fms, MSLL fms, MSAllocC fms, MSCache fms) in
     ms <- LOG.flushall_noop lxp ms;
-    Ret (mk_memstate (negb al) ms cache).
+    Ret (mk_memstate (negb al) ms alc cache).
 
   Definition pick_balloc A (a : A * A) (flag : bool) :=
     if flag then fst a else snd a.
@@ -150,76 +154,76 @@ Module BFILE.
   Qed.
 
   Definition grow lxp bxps ixp inum v fms :=
-    let '(al, ms, cache) := (MSAlloc fms, MSLL fms, MSCache fms) in
+    let '(al, ms, alc, cache) := (MSAlloc fms, MSLL fms, MSAllocC fms, MSCache fms) in
     let^ (ms, len) <- INODE.getlen lxp ixp inum ms;
     If (lt_dec len INODE.NBlocks) {
       let^ (ms, r) <- BALLOC.alloc lxp (pick_balloc bxps al) ms;
       match r with
-      | None => Ret ^(mk_memstate al ms cache, Err ENOSPCBLOCK)
+      | None => Ret ^(mk_memstate al ms alc cache, Err ENOSPCBLOCK)
       | Some bn =>
-           let^ (ms, succ) <- INODE.grow lxp (pick_balloc bxps al) ixp inum bn ms;
+           let^ (cms, succ) <- INODE.grow lxp (pick_balloc bxps al) ixp inum bn (BALLOCC.mk_memstate ms (pick_balloc alc al));
            match succ with
            | Err e =>
-             Ret ^(mk_memstate al ms cache, Err e)
+             Ret ^(mk_memstate al (BALLOCC.MSLog cms) (upd_balloc alc (BALLOCC.MSCache cms) al) cache, Err e)
            | OK _ =>
              ms <- LOG.write lxp bn v ms;
-             Ret ^(mk_memstate al ms cache, OK tt)
+             Ret ^(mk_memstate al  (BALLOCC.MSLog cms) (upd_balloc alc (BALLOCC.MSCache cms) al) cache, OK tt)
            end
       end
     } else {
-      Ret ^(mk_memstate al ms cache, Err EFBIG)
+      Ret ^(mk_memstate al ms alc cache, Err EFBIG)
     }.
 
   Definition shrink lxp bxps ixp inum nr fms :=
-    let '(al, ms, cache) := (MSAlloc fms, MSLL fms, MSCache fms) in
+    let '(al, ms, alc, cache) := (MSAlloc fms, MSLL fms, MSAllocC fms, MSCache fms) in
     let^ (ms, bns) <- INODE.getallbnum lxp ixp inum ms;
     let l := map (@wordToNat _) (skipn ((length bns) - nr) bns) in
-    ms <- BALLOC.freevec lxp (pick_balloc bxps (negb al)) l ms;
-    ms <- INODE.shrink lxp (pick_balloc bxps (negb al)) ixp inum nr ms;
-    Ret (mk_memstate al ms cache).
+    cms <- BALLOCC.freevec lxp (pick_balloc bxps (negb al)) l (BALLOCC.mk_memstate ms (pick_balloc alc al));
+    cms <- INODE.shrink lxp (pick_balloc bxps (negb al)) ixp inum nr cms;
+    Ret (mk_memstate al ms alc cache).
 
-  Definition shuffle_allocs lxp bxps ms :=
-    let^ (ms) <- ForN i < (BmapNBlocks (fst bxps) * valulen)
+  Definition shuffle_allocs lxp bxps ms cms :=
+    let^ (ms, cms) <- ForN i < (BmapNBlocks (fst bxps) * valulen)
     Hashmap hm
     Ghost [ F Fm crash m0 ]
-    Loopvar [ ms ]
+    Loopvar [ ms cms ]
     Invariant
          exists m' frees,
          LOG.rep lxp F (LOG.ActiveTxn m0 m') ms hm *
-         [[[ m' ::: (Fm * BALLOC.rep (fst bxps) (fst frees) *
-                         BALLOC.rep (snd bxps) (snd frees)) ]]] *
+         [[[ m' ::: (Fm * BALLOCC.rep (fst bxps) (fst frees) (BALLOCC.mk_memstate ms (fst cms))   *
+                         BALLOCC.rep (snd bxps) (snd frees) (BALLOCC.mk_memstate ms (snd cms))) ]]] *
          [[ forall bn, bn < (BmapNBlocks (fst bxps)) * valulen /\ bn >= i
              -> In bn (fst frees) ]]
     OnCrash crash
     Begin
       If (bool_dec (Nat.odd i) true) {
-        ms <- BALLOC.steal lxp (fst bxps) i ms;
-        ms <- BALLOC.free lxp (snd bxps) i ms;
-        Ret ^(ms)
+        fcms <- BALLOCC.steal lxp (fst bxps) i (BALLOCC.mk_memstate ms (fst cms));
+        scms <- BALLOCC.free lxp (snd bxps) i (BALLOCC.mk_memstate (BALLOCC.MSLog fcms) (snd cms));
+        Ret ^((BALLOCC.MSLog scms), ((BALLOCC.MSCache fcms), (BALLOCC.MSCache scms)))
       } else {
-        Ret ^(ms)
+        Ret ^(ms, cms)
       }
-    Rof ^(ms);
-    Ret ms.
+    Rof ^(ms, cms);
+    Ret ^(ms, cms).
 
   Definition init lxp bxps bixp ixp ms :=
-    ms <- BALLOC.init_nofree lxp (snd bxps) ms;
-    ms <- BALLOC.init lxp (fst bxps) ms;
-    ms <- IAlloc.init lxp bixp ms;
+    fcms <- BALLOCC.init_nofree lxp (snd bxps) ms;
+    scms <- BALLOCC.init lxp (fst bxps) (BALLOCC.MSLog fcms);
+    ms <- IAlloc.init lxp bixp (BALLOCC.MSLog scms);
     ms <- INODE.init lxp ixp ms;
-    ms <- shuffle_allocs lxp bxps ms;
-    Ret (mk_memstate true ms (BFcache.empty _)).
+    let^ (ms, cms) <- shuffle_allocs lxp bxps ms (BALLOCC.MSCache scms, BALLOCC.MSCache fcms);
+    Ret (mk_memstate true ms cms (BFcache.empty _)).
 
   Definition recover ms :=
-    Ret (mk_memstate true ms (BFcache.empty _)).
+    Ret (mk_memstate true ms (BALLOCC.Alloc.freelist0, BALLOCC.Alloc.freelist0)  (BFcache.empty _)).
 
   Definition cache_get inum fms :=
-    let '(al, ms, cache) := (MSAlloc fms, MSLL fms, MSCache fms) in
-    Ret ^(mk_memstate al ms cache, BFcache.find inum cache).
+    let '(al, ms, alc, cache) := (MSAlloc fms, MSLL fms, MSAllocC fms, MSCache fms) in
+    Ret ^(mk_memstate al ms alc cache, BFcache.find inum cache).
 
   Definition cache_put inum dc fms :=
-    let '(al, ms, cache) := (MSAlloc fms, MSLL fms, MSCache fms) in
-    Ret (mk_memstate al ms (BFcache.add inum dc cache)).
+    let '(al, ms, alc, cache) := (MSAlloc fms, MSLL fms, MSAllocC fms, MSCache fms) in
+    Ret (mk_memstate al ms alc (BFcache.add inum dc cache)).
 
 
   (* rep invariants *)
@@ -251,39 +255,42 @@ Module BFILE.
   Definition cache_rep mscache (flist : list bfile) (ilist : list INODE.inode) :=
      arrayN cache_ptsto 0 (map BFCache flist) (BFM.mm _ mscache).
 
-  Definition rep (bxps : balloc_xparams * balloc_xparams) ixp (flist : list bfile) ilist frees mscache :=
-    (BALLOC.rep (fst bxps) (fst frees) *
-     BALLOC.rep (snd bxps) (snd frees) *
+  Definition rep (bxps : balloc_xparams * balloc_xparams) ixp (flist : list bfile) ilist frees cms mscache :=
+    (exists lms, 
+     BALLOCC.rep (fst bxps) (fst frees) (BALLOCC.mk_memstate lms (fst cms)) *
+     BALLOCC.rep (snd bxps) (snd frees) (BALLOCC.mk_memstate lms (snd cms)) *
      INODE.rep (fst bxps) ixp ilist *
      listmatch file_match flist ilist *
      [[ locked (cache_rep mscache flist ilist) ]] *
      [[ BmapNBlocks (fst bxps) = BmapNBlocks (snd bxps) ]]
     )%pred.
 
-  Definition rep_length_pimpl : forall bxps ixp flist ilist frees mscache,
-    rep bxps ixp flist ilist frees mscache =p=>
-    (rep bxps ixp flist ilist frees mscache *
+  Definition rep_length_pimpl : forall bxps ixp flist ilist frees allocc mscache,
+    rep bxps ixp flist ilist frees allocc mscache =p=>
+    (rep bxps ixp flist ilist frees allocc mscache *
      [[ length flist = ((INODE.IRecSig.RALen ixp) * INODE.IRecSig.items_per_val)%nat ]] *
      [[ length ilist = ((INODE.IRecSig.RALen ixp) * INODE.IRecSig.items_per_val)%nat ]])%pred.
   Proof.
     unfold rep; intros.
+    norm'l; unfold stars; simpl.
     rewrite INODE.rep_length_pimpl at 1.
     rewrite listmatch_length_pimpl at 1.
     cancel.
   Qed.
 
   Definition rep_alt (bxps : BALLOC.Alloc.BmpSig.xparams * BALLOC.Alloc.BmpSig.xparams)
-                     ixp (flist : list bfile) ilist frees mscache msalloc :=
-    (BALLOC.rep (pick_balloc bxps msalloc)        (pick_balloc frees msalloc) *
-     BALLOC.rep (pick_balloc bxps (negb msalloc)) (pick_balloc frees (negb msalloc)) *
+                     ixp (flist : list bfile) ilist frees cms mscache msalloc :=
+    (exists lms,
+      BALLOCC.rep (pick_balloc bxps msalloc) (pick_balloc frees msalloc) (BALLOCC.mk_memstate lms (pick_balloc cms msalloc)) *
+     BALLOCC.rep (pick_balloc bxps (negb msalloc)) (pick_balloc frees (negb msalloc)) (BALLOCC.mk_memstate lms (pick_balloc cms (negb msalloc))) *
      INODE.rep (pick_balloc bxps msalloc) ixp ilist *
      listmatch file_match flist ilist *
      [[ locked (cache_rep mscache flist ilist) ]] *
      [[ BmapNBlocks (pick_balloc bxps msalloc) = BmapNBlocks (pick_balloc bxps (negb msalloc)) ]]
     )%pred.
 
-  Theorem rep_alt_equiv : forall bxps ixp flist ilist frees mscache msalloc,
-    rep bxps ixp flist ilist frees mscache <=p=> rep_alt bxps ixp flist ilist frees mscache msalloc.
+  Theorem rep_alt_equiv : forall bxps ixp flist ilist frees mscache allocc msalloc,
+    rep bxps ixp flist ilist frees allocc mscache <=p=> rep_alt bxps ixp flist ilist frees allocc mscache msalloc.
   Proof.
     unfold rep, rep_alt; split; destruct msalloc; simpl.
     - cancel.
@@ -306,8 +313,8 @@ Module BFILE.
     { block_is_unused freeblocks bn } + { ~ block_is_unused freeblocks bn }
     := In_dec addr_eq_dec bn freeblocks.
 
-  Lemma block_is_unused_xor_belong_to_file : forall F Ftop fsxp files ilist free mscache m flag bn inum off,
-    (F * rep fsxp Ftop files ilist free mscache)%pred m ->
+  Lemma block_is_unused_xor_belong_to_file : forall F Ftop fsxp files ilist free allocc mscache m flag bn inum off,
+    (F * rep fsxp Ftop files ilist free allocc mscache)%pred m ->
     block_is_unused (pick_balloc free flag) bn ->
     block_belong_to_file ilist bn inum off ->
     False.
@@ -319,11 +326,12 @@ Module BFILE.
     unfold file_match at 2 in H.
     erewrite listmatch_isolate with (i := off) (a := (BFData files ⟦ inum ⟧)) in H by simplen.
     erewrite selN_map in H; eauto.
-    unfold BALLOC.rep in H; destruct_lift H.
-    unfold BALLOC.Alloc.rep in H; destruct_lift H.
+    unfold BALLOCC.rep in H; destruct_lift H.
+    unfold BALLOCC.Alloc.rep in H; destruct_lift H.
+    unfold BALLOCC.Alloc.Alloc.rep in H; destruct_lift H.
     destruct flag; simpl in *.
-    - destruct H16 as [H16 _]. rewrite listpred_pick in H16 by eauto.
-      rewrite H16 in H.
+    - destruct H20 as [H20 _]. rewrite listpred_pick in H20 by eauto.
+      rewrite H20 in H.
       destruct_lift H.
       rewrite locked_eq in H3.
       rewrite <- H3 in H; clear H3.
@@ -331,8 +339,8 @@ Module BFILE.
       pred_apply.
       destruct ((BFData files ⟦ inum ⟧) ⟦ off ⟧).
       cancel.
-    - destruct H19 as [H19 _]. rewrite listpred_pick in H19 by eauto.
-      rewrite H19 in H.
+    - destruct H23 as [H23 _]. rewrite listpred_pick in H23 by eauto.
+      rewrite H23 in H.
       destruct_lift H.
       rewrite locked_eq in H3.
       rewrite <- H3 in H; clear H3.
@@ -406,8 +414,8 @@ Module BFILE.
     auto.
   Qed.
 
-  Theorem rep_used_block_eq : forall F bxps ixp flist ilist m bn inum off frees mscache,
-    (F * rep bxps ixp flist ilist frees mscache)%pred (list2nmem m) ->
+  Theorem rep_used_block_eq : forall F bxps ixp flist ilist m bn inum off frees allocc mscache,
+    (F * rep bxps ixp flist ilist frees allocc mscache)%pred (list2nmem m) ->
     block_belong_to_file ilist bn inum off ->
     selN (BFData (selN flist inum bfile0)) off ($0, nil) = selN m bn ($0, nil).
   Proof.
@@ -446,13 +454,13 @@ Module BFILE.
     all: eauto.
   Qed.
 
-  Theorem rep_safe_used: forall F bxps ixp flist ilist m bn inum off frees mscache v,
-    (F * rep bxps ixp flist ilist frees mscache)%pred (list2nmem m) ->
+  Theorem rep_safe_used: forall F bxps ixp flist ilist m bn inum off frees allocc mscache v,
+    (F * rep bxps ixp flist ilist frees allocc mscache)%pred (list2nmem m) ->
     block_belong_to_file ilist bn inum off ->
     let f := selN flist inum bfile0 in
     let f' := mk_bfile (updN (BFData f) off v) (BFAttr f) (BFCache f) in
     let flist' := updN flist inum f' in
-    (F * rep bxps ixp flist' ilist frees mscache)%pred (list2nmem (updN m bn v)).
+    (F * rep bxps ixp flist' ilist frees allocc mscache)%pred (list2nmem (updN m bn v)).
   Proof.
     unfold rep; intros.
     destruct_lift H.
@@ -514,16 +522,17 @@ Module BFILE.
     all: try exact None.
   Qed.
 
-  Theorem rep_safe_unused: forall F bxps ixp flist ilist m frees mscache bn v flag,
-    (F * rep bxps ixp flist ilist frees mscache)%pred (list2nmem m) ->
+  Theorem rep_safe_unused: forall F bxps ixp flist ilist m frees allocc mscache bn v flag,
+    (F * rep bxps ixp flist ilist frees allocc mscache)%pred (list2nmem m) ->
     block_is_unused (pick_balloc frees flag) bn ->
-    (F * rep bxps ixp flist ilist frees mscache)%pred (list2nmem (updN m bn v)).
+    (F * rep bxps ixp flist ilist frees allocc mscache)%pred (list2nmem (updN m bn v)).
   Proof.
     unfold rep, pick_balloc, block_is_unused; intros.
     destruct_lift H.
     destruct flag.
-    - unfold BALLOC.rep at 1 in H.
-      unfold BALLOC.Alloc.rep in H.
+    - unfold BALLOCC.rep at 1 in H.
+      unfold BALLOCC.Alloc.rep in H.
+      unfold BALLOCC.Alloc.Alloc.rep in H.
       destruct_lift H.
 
       denote listpred as Hx.
@@ -543,14 +552,15 @@ Module BFILE.
       rewrite Hy in H.
       destruct_lift H.
       eapply pimpl_trans; [ apply pimpl_refl | | eapply list2nmem_updN; pred_apply; cancel ].
-      unfold BALLOC.rep at 2. unfold BALLOC.Alloc.rep.
+      unfold BALLOCC.rep at 2. unfold BALLOCC.Alloc.rep. unfold BALLOCC.Alloc.Alloc.rep.
 
       norm; unfold stars; simpl.
       2: intuition eauto.
       cancel. rewrite Hy. cancel.
 
-    - unfold BALLOC.rep at 2 in H.
-      unfold BALLOC.Alloc.rep in H.
+    - unfold BALLOCC.rep at 2 in H.
+      unfold BALLOCC.Alloc.rep in H.
+      unfold BALLOCC.Alloc.Alloc.rep in H.
       destruct_lift H.
 
       denote listpred as Hx.
@@ -570,7 +580,7 @@ Module BFILE.
       rewrite Hy in H.
       destruct_lift H.
       eapply pimpl_trans; [ apply pimpl_refl | | eapply list2nmem_updN; pred_apply; cancel ].
-      unfold BALLOC.rep at 3. unfold BALLOC.Alloc.rep.
+      unfold BALLOCC.rep at 3. unfold BALLOCC.Alloc.rep. unfold BALLOCC.Alloc.Alloc.rep.
 
       norm; unfold stars; simpl.
       2: intuition eauto.
@@ -580,8 +590,8 @@ Module BFILE.
     all: apply addr_eq_dec.
   Qed.
 
-  Theorem block_belong_to_file_bfdata_length : forall bxp ixp flist ilist frees mscache m F inum off bn,
-    (F * rep bxp ixp flist ilist frees mscache)%pred m ->
+  Theorem block_belong_to_file_bfdata_length : forall bxp ixp flist ilist frees allocc mscache m F inum off bn,
+    (F * rep bxp ixp flist ilist frees allocc mscache)%pred m ->
     block_belong_to_file ilist bn inum off ->
     off < length (BFData (selN flist inum BFILE.bfile0)).
   Proof.
@@ -875,28 +885,28 @@ Module BFILE.
   Ltac assignms :=
     match goal with
     [ fms : memstate |- LOG.rep _ _ _ ?ms _ =p=> LOG.rep _ _ _ (MSLL ?e) _ ] =>
-      is_evar e; eassign (mk_memstate (MSAlloc fms) ms (MSCache fms)); simpl; eauto
+      is_evar e; eassign (mk_memstate (MSAlloc fms) ms (MSAllocC fms) (MSCache fms)); simpl; eauto
     end.
 
-  Local Hint Extern 1 (LOG.rep _ _ _ ?ms _ =p=> LOG.rep _ _ _ (MSLL ?e) _) => assignms.
+  Local Hint Extern 1 (LOG.rep _ _ _ ?ms _  =p=> LOG.rep _ _ _ (MSLL ?e) _ ) => assignms.
 
   (*** specification *)
 
 
-  Theorem shuffle_allocs_ok : forall lxp bxps ms,
+  Theorem shuffle_allocs_ok : forall lxp bxps ms cms,
     {< F Fm m0 m frees,
     PRE:hm
            LOG.rep lxp F (LOG.ActiveTxn m0 m) ms hm *
-           [[[ m ::: (Fm * BALLOC.rep (fst bxps) (fst frees) *
-                           BALLOC.rep (snd bxps) (snd frees)) ]]] *
+           [[[ m ::: (Fm * BALLOCC.rep (fst bxps) (fst frees) (BALLOCC.mk_memstate ms (fst cms)) *
+                           BALLOCC.rep (snd bxps) (snd frees) (BALLOCC.mk_memstate ms (snd cms))) ]]] *
            [[ forall bn, bn < (BmapNBlocks (fst bxps)) * valulen -> In bn (fst frees) ]] *
            [[ BmapNBlocks (fst bxps) = BmapNBlocks (snd bxps) ]]
-    POST:hm' RET:ms'  exists m' frees',
+    POST:hm' RET:^(ms',cms')  exists m' frees',
            LOG.rep lxp F (LOG.ActiveTxn m0 m') ms' hm' *
-           [[[ m' ::: (Fm * BALLOC.rep (fst bxps) (fst frees') *
-                            BALLOC.rep (snd bxps) (snd frees')) ]]]
+           [[[ m' ::: (Fm * BALLOCC.rep (fst bxps) (fst frees') (BALLOCC.mk_memstate ms' (fst cms')) *
+                            BALLOCC.rep (snd bxps) (snd frees') (BALLOCC.mk_memstate ms' (snd cms'))) ]]]
     CRASH:hm'  LOG.intact lxp F m0 hm'
-    >} shuffle_allocs lxp bxps ms.
+    >} shuffle_allocs lxp bxps ms cms.
   Proof.
     unfold shuffle_allocs.
     step.
@@ -917,7 +927,7 @@ Module BFILE.
     Unshelve. exact tt.
   Qed.
 
-  Hint Extern 1 ({{_}} Bind (shuffle_allocs _ _ _) _) => apply shuffle_allocs_ok : prog.
+  Hint Extern 1 ({{_}} Bind (shuffle_allocs _ _ _ _) _) => apply shuffle_allocs_ok : prog.
 
   Local Hint Resolve INODE.IRec.Defs.items_per_val_gt_0 INODE.IRec.Defs.items_per_val_not_0 valulen_gt_0.
 
@@ -943,9 +953,9 @@ Module BFILE.
               data_bitmaps <= valulen * valulen /\
              inode_bitmaps <= valulen * valulen
            ]]
-    POST:hm' RET:ms'  exists m' n frees freeinodes freeinode_pred,
+    POST:hm' RET:ms'  exists m' n frees allocc freeinodes freeinode_pred,
            LOG.rep lxp F (LOG.ActiveTxn m0 m') (MSLL ms') hm' *
-           [[[ m' ::: (Fm * rep bxps ixp (repeat bfile0 n) (repeat INODE.inode0 n) frees (MSCache ms') * 
+           [[[ m' ::: (Fm * rep bxps ixp (repeat bfile0 n) (repeat INODE.inode0 n) allocc frees (MSCache ms') * 
                             @IAlloc.rep bfile freepred ibxp freeinodes freeinode_pred) ]]] *
            [[ n = ((IXLen ixp) * INODE.IRecSig.items_per_val)%nat /\ n > 1 ]] *
            [[ forall dl, length dl = n ->
@@ -1046,10 +1056,10 @@ Module BFILE.
   Qed.
 
   Theorem getlen_ok : forall lxp bxps ixp inum ms,
-    {< F Fm Fi m0 m f flist ilist frees,
+    {< F Fm Fi m0 m f flist ilist allocc frees,
     PRE:hm
            LOG.rep lxp F (LOG.ActiveTxn m0 m) (MSLL ms) hm *
-           [[[ m ::: (Fm * rep bxps ixp flist ilist frees (MSCache ms)) ]]] *
+           [[[ m ::: (Fm * rep bxps ixp flist ilist frees allocc (MSCache ms)) ]]] *
            [[[ flist ::: (Fi * inum |-> f) ]]]
     POST:hm' RET:^(ms',r)
            LOG.rep lxp F (LOG.ActiveTxn m0 m) (MSLL ms') hm' *
@@ -1075,10 +1085,10 @@ Module BFILE.
   Qed.
 
   Theorem getattrs_ok : forall lxp bxp ixp inum ms,
-    {< F Fm Fi m0 m flist ilist frees f,
+    {< F Fm Fi m0 m flist ilist allocc frees f,
     PRE:hm
            LOG.rep lxp F (LOG.ActiveTxn m0 m) (MSLL ms) hm *
-           [[[ m ::: (Fm * rep bxp ixp flist ilist frees (MSCache ms)) ]]] *
+           [[[ m ::: (Fm * rep bxp ixp flist ilist  frees allocc (MSCache ms)) ]]] *
            [[[ flist ::: (Fi * inum |-> f) ]]]
     POST:hm' RET:^(ms',r)
            LOG.rep lxp F (LOG.ActiveTxn m0 m) (MSLL ms') hm' *
@@ -1124,14 +1134,14 @@ Module BFILE.
   Qed.
 
   Theorem setattrs_ok : forall lxp bxps ixp inum a ms,
-    {< F Fm Ff m0 m flist ilist frees f,
+    {< F Fm Ff m0 m flist ilist allocc frees f,
     PRE:hm
            LOG.rep lxp F (LOG.ActiveTxn m0 m) (MSLL ms) hm *
-           [[[ m ::: (Fm * rep bxps ixp flist ilist frees (MSCache ms)) ]]] *
+           [[[ m ::: (Fm * rep bxps ixp flist ilist frees allocc (MSCache ms)) ]]] *
            [[[ flist ::: (Ff * inum |-> f) ]]] 
     POST:hm' RET:ms'  exists m' flist' f' ilist',
            LOG.rep lxp F (LOG.ActiveTxn m0 m') (MSLL ms') hm' *
-           [[[ m' ::: (Fm * rep bxps ixp flist' ilist' frees (MSCache ms')) ]]] *
+           [[[ m' ::: (Fm * rep bxps ixp flist' ilist' frees allocc (MSCache ms')) ]]] *
            [[[ flist' ::: (Ff * inum |-> f') ]]] *
            [[ f' = mk_bfile (BFData f) a (BFCache f) ]] *
            [[ MSAlloc ms = MSAlloc ms' /\
@@ -1182,14 +1192,14 @@ Module BFILE.
   Qed.
 
   Theorem updattr_ok : forall lxp bxps ixp inum kv ms,
-    {< F Fm Fi m0 m flist ilist frees f,
+    {< F Fm Fi m0 m flist ilist frees allocc f,
     PRE:hm
            LOG.rep lxp F (LOG.ActiveTxn m0 m) (MSLL ms) hm *
-           [[[ m ::: (Fm * rep bxps ixp flist ilist frees (MSCache ms)) ]]] *
+           [[[ m ::: (Fm * rep bxps ixp flist ilist frees allocc (MSCache ms)) ]]] *
            [[[ flist ::: (Fi * inum |-> f) ]]]
     POST:hm' RET:ms'  exists m' flist' ilist' f',
            LOG.rep lxp F (LOG.ActiveTxn m0 m') (MSLL ms') hm' *
-           [[[ m' ::: (Fm * rep bxps ixp flist' ilist' frees (MSCache ms')) ]]] *
+           [[[ m' ::: (Fm * rep bxps ixp flist' ilist' frees allocc (MSCache ms')) ]]] *
            [[[ flist' ::: (Fi * inum |-> f') ]]] *
            [[ f' = mk_bfile (BFData f) (INODE.iattr_upd (BFAttr f) kv) (BFCache f) ]] *
            [[ MSAlloc ms = MSAlloc ms' /\
@@ -1225,11 +1235,11 @@ Module BFILE.
   Qed.
 
   Theorem read_ok : forall lxp bxp ixp inum off ms,
-    {< F Fm Fi Fd m0 m flist ilist frees f vs,
+    {< F Fm Fi Fd m0 m flist ilist frees allocc f vs,
     PRE:hm
            LOG.rep lxp F (LOG.ActiveTxn m0 m) (MSLL ms) hm *
            [[ off < length (BFData f) ]] *
-           [[[ m ::: (Fm * rep bxp ixp flist ilist frees (MSCache ms)) ]]] *
+           [[[ m ::: (Fm * rep bxp ixp flist ilist frees allocc (MSCache ms)) ]]] *
            [[[ flist ::: (Fi * inum |-> f) ]]] *
            [[[ (BFData f) ::: (Fd * off |-> vs) ]]]
     POST:hm' RET:^(ms', r)
@@ -1265,16 +1275,16 @@ Module BFILE.
 
 
   Theorem write_ok : forall lxp bxp ixp inum off v ms,
-    {< F Fm Fi Fd m0 m flist ilist frees f vs0,
+    {< F Fm Fi Fd m0 m flist ilist frees allocc f vs0,
     PRE:hm
            LOG.rep lxp F (LOG.ActiveTxn m0 m) (MSLL ms) hm *
            [[ off < length (BFData f) ]] *
-           [[[ m ::: (Fm * rep bxp ixp flist ilist frees (MSCache ms)) ]]] *
+           [[[ m ::: (Fm * rep bxp ixp flist ilist frees allocc (MSCache ms)) ]]] *
            [[[ flist ::: (Fi * inum |-> f) ]]] *
            [[[ (BFData f) ::: (Fd * off |-> vs0) ]]]
     POST:hm' RET:ms'  exists m' flist' f',
            LOG.rep lxp F (LOG.ActiveTxn m0 m') (MSLL ms') hm' *
-           [[[ m' ::: (Fm * rep bxp ixp flist' ilist frees (MSCache ms')) ]]] *
+           [[[ m' ::: (Fm * rep bxp ixp flist' ilist frees allocc (MSCache ms')) ]]] *
            [[[ flist' ::: (Fi * inum |-> f') ]]] *
            [[[ (BFData f') ::: (Fd * off |-> (v, nil)) ]]] *
            [[ f' = mk_bfile (updN (BFData f) off (v, nil)) (BFAttr f) (BFCache f) ]] *
@@ -1357,14 +1367,14 @@ Module BFILE.
     {< F Fm Fi Fd m0 m flist ilist frees f,
     PRE:hm
            LOG.rep lxp F (LOG.ActiveTxn m0 m) (MSLL ms) hm *
-           [[[ m ::: (Fm * rep bxp ixp flist ilist frees (MSCache ms)) ]]] *
+           [[[ m ::: (Fm * rep bxp ixp flist ilist frees (MSAllocC ms) (MSCache ms)) ]]] *
            [[[ flist ::: (Fi * inum |-> f) ]]] *
            [[[ (BFData f) ::: Fd ]]]
     POST:hm' RET:^(ms', r) [[ MSAlloc ms = MSAlloc ms' /\ MSCache ms = MSCache ms' ]] * exists m',
            [[ isError r ]] * LOG.rep lxp F (LOG.ActiveTxn m0 m') (MSLL ms') hm' \/
            [[ r = OK tt  ]] * exists flist' ilist' frees' f',
            LOG.rep lxp F (LOG.ActiveTxn m0 m') (MSLL ms') hm' *
-           [[[ m' ::: (Fm * rep bxp ixp flist' ilist' frees' (MSCache ms')) ]]] *
+           [[[ m' ::: (Fm * rep bxp ixp flist' ilist' frees' (MSAllocC ms') (MSCache ms')) ]]] *
            [[[ flist' ::: (Fi * inum |-> f') ]]] *
            [[[ (BFData f') ::: (Fd * (length (BFData f)) |-> (v, nil)) ]]] *
            [[ f' = mk_bfile ((BFData f) ++ [(v, nil)]) (BFAttr f) (BFCache f) ]] *
@@ -1460,11 +1470,11 @@ Module BFILE.
     {< F Fm Fi m0 m flist ilist frees f,
     PRE:hm
            LOG.rep lxp F (LOG.ActiveTxn m0 m) (MSLL ms) hm *
-           [[[ m ::: (Fm * rep bxp ixp flist ilist frees (MSCache ms)) ]]] *
+           [[[ m ::: (Fm * rep bxp ixp flist ilist frees (MSAllocC ms) (MSCache ms)) ]]] *
            [[[ flist ::: (Fi * inum |-> f) ]]]
     POST:hm' RET:ms'  exists m' flist' f' ilist' frees',
            LOG.rep lxp F (LOG.ActiveTxn m0 m') (MSLL ms') hm' *
-           [[[ m' ::: (Fm * rep bxp ixp flist' ilist' frees' (MSCache ms')) ]]] *
+           [[[ m' ::: (Fm * rep bxp ixp flist' ilist' frees' (MSAllocC ms') (MSCache ms')) ]]] *
            [[[ flist' ::: (Fi * inum |-> f') ]]] *
            [[ f' = mk_bfile (firstn ((length (BFData f)) - nr) (BFData f)) (BFAttr f) (BFCache f) ]] *
            [[ MSCache ms = MSCache ms' ]] *
@@ -1581,7 +1591,8 @@ Module BFILE.
     POST:hm' RET:ms'
       LOG.rep lxp F (LOG.NoTxn (ds!!, nil)) (MSLL ms') hm' *
       [[ MSAlloc ms' = negb (MSAlloc ms) ]] *
-      [[ MSCache ms' = MSCache ms ]]
+      [[ MSCache ms' = MSCache ms ]] *
+      [[ MSAllocC ms' = MSAllocC ms]]
     XCRASH:hm'
       LOG.recover_any lxp F ds hm'
     >} sync lxp ixp ms.
@@ -1599,7 +1610,8 @@ Module BFILE.
     POST:hm' RET:ms'
       LOG.rep lxp F (LOG.NoTxn ds) (MSLL ms') hm' *
       [[ MSAlloc ms' = negb (MSAlloc ms) ]] *
-      [[ MSCache ms' = MSCache ms ]]
+      [[ MSCache ms' = MSCache ms ]] *
+      [[ MSAllocC ms' = MSAllocC ms]]
     XCRASH:hm'
       LOG.recover_any lxp F ds hm'
     >} sync_noop lxp ixp ms.
@@ -1609,8 +1621,8 @@ Module BFILE.
     step.
   Qed.
 
-  Lemma block_belong_to_file_off_ok : forall Fm Fi bxp ixp flist ilist frees mscache inum off f m,
-    (Fm * rep bxp ixp flist ilist frees mscache)%pred m ->
+  Lemma block_belong_to_file_off_ok : forall Fm Fi bxp ixp flist ilist frees cms mscache inum off f m,
+    (Fm * rep bxp ixp flist ilist frees cms mscache)%pred m ->
     (Fi * inum |-> f)%pred (list2nmem flist) ->
     off < Datatypes.length (BFData f) -> 
     block_belong_to_file ilist # (selN (INODE.IBlocks (selN ilist inum INODE.inode0)) off $0) inum off.
@@ -1627,8 +1639,8 @@ Module BFILE.
     Unshelve. eauto.
   Qed.
 
-  Lemma block_belong_to_file_ok : forall Fm Fi Fd bxp ixp flist ilist frees mscache inum off f vs m,
-    (Fm * rep bxp ixp flist ilist frees mscache)%pred m ->
+  Lemma block_belong_to_file_ok : forall Fm Fi Fd bxp ixp flist ilist frees cms mscache inum off f vs m,
+    (Fm * rep bxp ixp flist ilist frees cms mscache)%pred m ->
     (Fi * inum |-> f)%pred (list2nmem flist) ->
     (Fd * off |-> vs)%pred (list2nmem (BFData f)) ->
     block_belong_to_file ilist # (selN (INODE.IBlocks (selN ilist inum INODE.inode0)) off $0) inum off.
@@ -1652,11 +1664,11 @@ Module BFILE.
   Qed.
 
   Theorem dwrite_ok : forall lxp bxp ixp inum off v ms,
-    {< F Fm Fi Fd ds flist ilist frees f vs,
+    {< F Fm Fi Fd ds flist ilist frees allocc f vs,
     PRE:hm
            LOG.rep lxp F (LOG.ActiveTxn ds ds!!) (MSLL ms) hm *
            [[ off < length (BFData f) ]] *
-           [[[ ds!! ::: (Fm  * rep bxp ixp flist ilist frees (MSCache ms)) ]]] *
+           [[[ ds!! ::: (Fm  * rep bxp ixp flist ilist frees allocc (MSCache ms)) ]]] *
            [[[ flist ::: (Fi * inum |-> f) ]]] *
            [[[ (BFData f) ::: (Fd * off |-> vs) ]]] *
            [[ sync_invariant F ]]
@@ -1666,7 +1678,7 @@ Module BFILE.
            [[ block_belong_to_file ilist bn inum off ]] *
            [[ MSAlloc ms = MSAlloc ms' ]] *
            (* spec about files on the latest diskset *)
-           [[[ ds'!! ::: (Fm  * rep bxp ixp flist' ilist frees (MSCache ms')) ]]] *
+           [[[ ds'!! ::: (Fm  * rep bxp ixp flist' ilist frees allocc (MSCache ms')) ]]] *
            [[[ flist' ::: (Fi * inum |-> f') ]]] *
            [[[ (BFData f') ::: (Fd * off |-> (v, vsmerge vs)) ]]] *
            [[ f' = mk_bfile (updN (BFData f) off (v, vsmerge vs)) (BFAttr f) (BFCache f) ]]
@@ -1734,16 +1746,16 @@ Module BFILE.
   Qed.
 
   Theorem datasync_ok : forall lxp bxp ixp inum ms,
-    {< F Fm Fi ds flist ilist free f,
+    {< F Fm Fi ds flist ilist free allocc f,
     PRE:hm
            LOG.rep lxp F (LOG.ActiveTxn ds ds!!) (MSLL ms) hm *
-           [[[ ds!!  ::: (Fm  * rep bxp ixp flist ilist free (MSCache ms)) ]]] *
+           [[[ ds!!  ::: (Fm  * rep bxp ixp flist ilist free allocc (MSCache ms)) ]]] *
            [[[ flist ::: (Fi * inum |-> f) ]]] *
            [[ sync_invariant F ]]
     POST:hm' RET:ms'  exists ds' flist' al,
            LOG.rep lxp F (LOG.ActiveTxn ds' ds'!!) (MSLL ms') hm' *
            [[ ds' = dssync_vecs ds al ]] *
-           [[[ ds'!! ::: (Fm * rep bxp ixp flist' ilist free (MSCache ms')) ]]] *
+           [[[ ds'!! ::: (Fm * rep bxp ixp flist' ilist free allocc (MSCache ms')) ]]] *
            [[[ flist' ::: (Fi * inum |-> synced_file f) ]]] *
            [[ MSAlloc ms = MSAlloc ms' ]] *
            [[ length al = length (BFILE.BFData f) /\ forall i, i < length al ->
@@ -1803,7 +1815,7 @@ Module BFILE.
   Hint Extern 1 ({{_}} Bind (datasync _ _ _ _) _) => apply datasync_ok : prog.
   Hint Extern 1 ({{_}} Bind (sync _ _ _) _) => apply sync_ok : prog.
   Hint Extern 1 ({{_}} Bind (sync_noop _ _ _) _) => apply sync_noop_ok : prog.
-  Hint Extern 0 (okToUnify (rep _ _ _ _ _ _) (rep _ _ _ _ _ _)) => constructor : okToUnify.
+  Hint Extern 0 (okToUnify (rep _ _ _ _ _ _ _) (rep _ _ _ _ _ _ _)) => constructor : okToUnify.
 
 
   Definition read_array lxp ixp inum a i ms :=
@@ -1815,10 +1827,10 @@ Module BFILE.
     Ret ms.
 
   Theorem read_array_ok : forall lxp bxp ixp inum a i ms,
-    {< F Fm Fi Fd m0 m flist ilist free f vsl,
+    {< F Fm Fi Fd m0 m flist ilist free allocc f vsl,
     PRE:hm
            LOG.rep lxp F (LOG.ActiveTxn m0 m) (MSLL ms) hm *
-           [[[ m ::: (Fm * rep bxp ixp flist ilist free (MSCache ms)) ]]] *
+           [[[ m ::: (Fm * rep bxp ixp flist ilist free allocc (MSCache ms)) ]]] *
            [[[ flist ::: (Fi * inum |-> f) ]]] *
            [[[ (BFData f) ::: Fd * arrayN (@ptsto _ addr_eq_dec _) a vsl ]]] *
            [[ i < length vsl]]
@@ -1843,21 +1855,22 @@ Module BFILE.
 
 
   Theorem write_array_ok : forall lxp bxp ixp inum a i v ms,
-    {< F Fm Fi Fd m0 m flist ilist free f vsl,
+    {< F Fm Fi Fd m0 m flist ilist free allocc f vsl,
     PRE:hm
            LOG.rep lxp F (LOG.ActiveTxn m0 m) (MSLL ms) hm *
-           [[[ m ::: (Fm * rep bxp ixp flist ilist free (MSCache ms)) ]]] *
+           [[[ m ::: (Fm * rep bxp ixp flist ilist free allocc (MSCache ms)) ]]] *
            [[[ flist ::: (Fi * inum |-> f) ]]] *
            [[[ (BFData f) ::: Fd * arrayN (@ptsto _ addr_eq_dec _) a vsl ]]] *
            [[ i < length vsl]]
     POST:hm' RET:ms' exists m' flist' f',
            LOG.rep lxp F (LOG.ActiveTxn m0 m') (MSLL ms') hm' *
-           [[[ m' ::: (Fm * rep bxp ixp flist' ilist free (MSCache ms')) ]]] *
+           [[[ m' ::: (Fm * rep bxp ixp flist' ilist free allocc (MSCache ms')) ]]] *
            [[[ flist' ::: (Fi * inum |-> f') ]]] *
            [[[ (BFData f') ::: Fd * arrayN (@ptsto _ addr_eq_dec _) a (updN vsl i (v, nil)) ]]] *
            [[ f' = mk_bfile (updN (BFData f) (a + i) (v, nil)) (BFAttr f) (BFCache f) ]] *
            [[ MSAlloc ms = MSAlloc ms' ]] *
-           [[ MSCache ms = MSCache ms' ]]
+           [[ MSCache ms = MSCache ms' ]] *
+           [[ MSAllocC ms = MSAllocC ms' ]]
     CRASH:hm'  LOG.intact lxp F m0 hm'
     >} write_array lxp ixp inum a i v ms.
   Proof.
@@ -1882,11 +1895,11 @@ Module BFILE.
   Definition read_range A lxp ixp inum a nr (vfold : A -> valu -> A) v0 ms0 :=
     let^ (ms, r) <- ForN i < nr
     Hashmap hm
-    Ghost [ bxp F Fm Fi Fd crash m0 m flist ilist frees f vsl ]
+    Ghost [ bxp F Fm Fi Fd crash m0 m flist ilist frees allocc f vsl ]
     Loopvar [ ms pf ]
     Invariant
       LOG.rep lxp F (LOG.ActiveTxn m0 m) (MSLL ms) hm *
-      [[[ m ::: (Fm * rep bxp ixp flist ilist frees (MSCache ms)) ]]] *
+      [[[ m ::: (Fm * rep bxp ixp flist ilist frees allocc (MSCache ms)) ]]] *
       [[[ flist ::: (Fi * inum |-> f) ]]] *
       [[[ (BFData f) ::: Fd * arrayN (@ptsto _ addr_eq_dec _) a vsl ]]] *
       [[ pf = fold_left vfold (firstn i (map fst vsl)) v0 ]] *
@@ -1901,10 +1914,10 @@ Module BFILE.
 
 
   Theorem read_range_ok : forall A lxp bxp ixp inum a nr (vfold : A -> valu -> A) v0 ms,
-    {< F Fm Fi Fd m0 m flist ilist frees f vsl,
+    {< F Fm Fi Fd m0 m flist ilist frees allocc f vsl,
     PRE:hm
            LOG.rep lxp F (LOG.ActiveTxn m0 m) (MSLL ms) hm *
-           [[[ m ::: (Fm * rep bxp ixp flist ilist frees (MSCache ms)) ]]] *
+           [[[ m ::: (Fm * rep bxp ixp flist ilist frees allocc (MSCache ms)) ]]] *
            [[[ flist ::: (Fi * inum |-> f) ]]] *
            [[[ (BFData f) ::: Fd * arrayN (@ptsto _ addr_eq_dec _) a vsl ]]] *
            [[ nr <= length vsl]]
@@ -1912,7 +1925,8 @@ Module BFILE.
            LOG.rep lxp F (LOG.ActiveTxn m0 m) (MSLL ms') hm' *
            [[ r = fold_left vfold (firstn nr (map fst vsl)) v0 ]] *
            [[ MSAlloc ms = MSAlloc ms' ]] *
-           [[ MSCache ms = MSCache ms' ]]
+           [[ MSCache ms = MSCache ms' ]] *
+           [[ MSAllocC ms = MSAllocC ms' ]]
     CRASH:hm'  exists ms',
            LOG.rep lxp F (LOG.ActiveTxn m0 m) (MSLL ms') hm'
     >} read_range lxp ixp inum a nr vfold v0 ms.
@@ -1944,11 +1958,11 @@ Module BFILE.
     let^ (ms, nr) <- getlen lxp ixp inum ms0;
     let^ (ms, r, ret) <- ForN i < nr
     Hashmap hm
-    Ghost [ bxp F Fm Fi m0 m flist f ilist frees ]
+    Ghost [ bxp F Fm Fi m0 m flist f ilist frees allocc ]
     Loopvar [ ms pf ret ]
     Invariant
       LOG.rep lxp F (LOG.ActiveTxn m0 m) (MSLL ms) hm *
-      [[[ m ::: (Fm * rep bxp ixp flist ilist frees (MSCache ms)) ]]] *
+      [[[ m ::: (Fm * rep bxp ixp flist ilist frees allocc (MSCache ms)) ]]] *
       [[[ flist ::: (Fi * inum |-> f) ]]] *
       [[ MSAlloc ms = MSAlloc ms0 ]] *
       [[ MSCache ms = MSCache ms0 ]] *
@@ -1978,16 +1992,17 @@ Module BFILE.
 
   Theorem read_cond_ok : forall A lxp bxp ixp inum (vfold : A -> valu -> A)
                                 v0 (cond : A -> bool) ms,
-    {< F Fm Fi m0 m flist ilist frees f,
+    {< F Fm Fi m0 m flist ilist frees allocc f,
     PRE:hm
            LOG.rep lxp F (LOG.ActiveTxn m0 m) (MSLL ms) hm *
-           [[[ m ::: (Fm * rep bxp ixp flist ilist frees (MSCache ms)) ]]] *
+           [[[ m ::: (Fm * rep bxp ixp flist ilist frees allocc (MSCache ms)) ]]] *
            [[[ flist ::: (Fi * inum |-> f) ]]] *
            [[ cond v0 = false ]]
     POST:hm' RET:^(ms', r)
            LOG.rep lxp F (LOG.ActiveTxn m0 m) (MSLL ms') hm' *
            [[ MSAlloc ms = MSAlloc ms' ]] *
            [[ MSCache ms = MSCache ms' ]] *
+           [[ MSAllocC ms = MSAllocC ms' ]] *
            ( exists v, 
              [[ r = Some v /\ cond v = true ]] \/
              [[ r = None /\ cond (fold_left vfold (map fst (BFData f)) v0) = false ]])
@@ -2042,7 +2057,7 @@ Module BFILE.
         ([[ isError ret ]] \/
          exists flist' ilist' frees' f',
          [[ ret = OK tt ]] *
-         [[[ m' ::: (Fm * rep bxp ixp flist' ilist' frees' (MSCache ms)) ]]] *
+         [[[ m' ::: (Fm * rep bxp ixp flist' ilist' frees' (MSAllocC ms) (MSCache ms)) ]]] *
          [[[ flist' ::: (Fi * inum |-> f') ]]] *
          [[  f' = mk_bfile ((BFData f) ++ synced_list (firstn i l)) (BFAttr f) (BFCache f) ]] *
          [[ ilist_safe ilist  (pick_balloc frees  (MSAlloc ms)) 
@@ -2067,7 +2082,7 @@ Module BFILE.
       ms <- shrink lxp bxp xp inum (sz - newsz) ms;
       Ret ^(ms, OK tt)
     } else {
-      let^ (ms, ok) <- grown lxp bxp xp inum (repeat $0 (newsz - sz))  ms;
+      let^ (ms, ok) <- grown lxp bxp xp inum (repeat $0 (newsz - sz)) ms;
       Ret ^(ms, ok)
     }.
 
@@ -2076,14 +2091,14 @@ Module BFILE.
     let^ (ms, sz) <- getlen lxp xp inum ms;
     ms <- shrink lxp bxp xp inum sz ms;
     ms <- setattrs lxp xp inum attr0 ms;
-    Ret (mk_memstate (MSAlloc ms) (MSLL ms) (BFcache.remove inum (MSCache ms))).
+    Ret (mk_memstate (MSAlloc ms) (MSLL ms) (MSAllocC ms) (BFcache.remove inum (MSCache ms))).
 
 
   Theorem grown_ok : forall lxp bxp ixp inum l ms,
     {< F Fm Fi Fd m0 m flist ilist frees f,
     PRE:hm
            LOG.rep lxp F (LOG.ActiveTxn m0 m) (MSLL ms) hm *
-           [[[ m ::: (Fm * rep bxp ixp flist ilist frees (MSCache ms)) ]]] *
+           [[[ m ::: (Fm * rep bxp ixp flist ilist frees (MSAllocC ms) (MSCache ms)) ]]] *
            [[[ flist ::: (Fi * inum |-> f) ]]] *
            [[[ (BFData f) ::: Fd ]]]
     POST:hm' RET:^(ms', r)
@@ -2093,7 +2108,7 @@ Module BFILE.
            [[ isError r ]] * LOG.rep lxp F (LOG.ActiveTxn m0 m') (MSLL ms') hm' \/
            [[ r = OK tt  ]] * exists flist' ilist' frees' f',
            LOG.rep lxp F (LOG.ActiveTxn m0 m') (MSLL ms') hm' *
-           [[[ m' ::: (Fm * rep bxp ixp flist' ilist' frees' (MSCache ms')) ]]] *
+           [[[ m' ::: (Fm * rep bxp ixp flist' ilist' frees' (MSAllocC ms') (MSCache ms')) ]]] *
            [[[ flist' ::: (Fi * inum |-> f') ]]] *
            [[[ (BFData f') ::: (Fd * arrayN (@ptsto _ addr_eq_dec _) (length (BFData f)) (synced_list l)) ]]] *
            [[ f' = mk_bfile ((BFData f) ++ (synced_list l)) (BFAttr f) (BFCache f) ]] *
@@ -2143,7 +2158,7 @@ Module BFILE.
     {< F Fm Fi m0 m flist ilist frees f,
     PRE:hm
            LOG.rep lxp F (LOG.ActiveTxn m0 m) (MSLL ms) hm *
-           [[[ m ::: (Fm * rep bxp ixp flist ilist frees (MSCache ms)) ]]] *
+           [[[ m ::: (Fm * rep bxp ixp flist ilist frees (MSAllocC ms) (MSCache ms)) ]]] *
            [[[ flist ::: (Fi * inum |-> f) ]]]
     POST:hm' RET:^(ms', r)
            [[ MSAlloc ms = MSAlloc ms' ]] *
@@ -2152,7 +2167,7 @@ Module BFILE.
            [[ isError r ]] * LOG.rep lxp F (LOG.ActiveTxn m0 m') (MSLL ms') hm' \/
            [[ r = OK tt  ]] * exists flist' ilist' frees' f',
            LOG.rep lxp F (LOG.ActiveTxn m0 m') (MSLL ms') hm' *
-           [[[ m' ::: (Fm * rep bxp ixp flist' ilist' frees' (MSCache ms')) ]]] *
+           [[[ m' ::: (Fm * rep bxp ixp flist' ilist' frees' (MSAllocC ms') (MSCache ms')) ]]] *
            [[[ flist' ::: (Fi * inum |-> f') ]]] *
            [[ f' = mk_bfile (setlen (BFData f) sz ($0, nil)) (BFAttr f) (BFCache f) ]] *
            [[ ilist_safe ilist (pick_balloc frees (MSAlloc ms')) 
@@ -2191,11 +2206,11 @@ Module BFILE.
     {< F Fm Fi m0 m flist ilist frees f,
     PRE:hm
            LOG.rep lxp F (LOG.ActiveTxn m0 m) (MSLL ms) hm *
-           [[[ m ::: (Fm * rep bxp ixp flist ilist frees (MSCache ms)) ]]] *
+           [[[ m ::: (Fm * rep bxp ixp flist ilist frees (MSAllocC ms) (MSCache ms)) ]]] *
            [[[ flist ::: (Fi * inum |-> f) ]]]
     POST:hm' RET:ms' exists m' flist' ilist' frees',
            LOG.rep lxp F (LOG.ActiveTxn m0 m') (MSLL ms') hm' *
-           [[[ m' ::: (Fm * rep bxp ixp flist' ilist' frees' (MSCache ms')) ]]] *
+           [[[ m' ::: (Fm * rep bxp ixp flist' ilist' frees' (MSAllocC ms') (MSCache ms')) ]]] *
            [[[ flist' ::: (Fi * inum |-> bfile0) ]]] *
            [[ MSAlloc ms = MSAlloc ms' /\ 
               ilist_safe ilist (pick_balloc frees (MSAlloc ms')) 
@@ -2232,10 +2247,10 @@ Module BFILE.
 
 
   Theorem cache_get_ok : forall inum ms,
-    {< F Fm Fi m0 m lxp bxp ixp flist ilist frees f,
+    {< F Fm Fi m0 m lxp bxp ixp flist ilist frees allocc f,
     PRE:hm
            LOG.rep lxp F (LOG.ActiveTxn m0 m) (MSLL ms) hm *
-           [[[ m ::: (Fm * rep bxp ixp flist ilist frees (MSCache ms)) ]]] *
+           [[[ m ::: (Fm * rep bxp ixp flist ilist frees allocc (MSCache ms)) ]]] *
            [[[ flist ::: (Fi * inum |-> f) ]]]
     POST:hm' RET:^(ms', r)
            [[ ms' = ms ]] *
@@ -2252,15 +2267,15 @@ Module BFILE.
   Qed.
 
   Theorem cache_put_ok : forall inum ms c,
-    {< F Fm Fi m0 m lxp bxp ixp flist ilist frees f,
+    {< F Fm Fi m0 m lxp bxp ixp flist ilist frees allocc f,
     PRE:hm
            LOG.rep lxp F (LOG.ActiveTxn m0 m) (MSLL ms) hm *
-           [[[ m ::: (Fm * rep bxp ixp flist ilist frees (MSCache ms)) ]]] *
+           [[[ m ::: (Fm * rep bxp ixp flist ilist frees allocc (MSCache ms)) ]]] *
            [[[ flist ::: (Fi * inum |-> f) ]]]
     POST:hm' RET:ms'
            exists f' flist',
            LOG.rep lxp F (LOG.ActiveTxn m0 m) (MSLL ms') hm *
-           [[[ m ::: (Fm * rep bxp ixp flist' ilist frees (MSCache ms')) ]]] *
+           [[[ m ::: (Fm * rep bxp ixp flist' ilist frees allocc (MSCache ms')) ]]] *
            [[[ flist' ::: (Fi * inum |-> f') ]]] *
            [[ f' = mk_bfile (BFData f) (BFAttr f) (Some c) ]]
     CRASH:hm'  LOG.intact lxp F m0 hm'
@@ -2437,10 +2452,10 @@ Module BFILE.
     simpl; omega.
   Qed.
 
-  Lemma xform_rep : forall bxp ixp flist ilist frees mscache,
-    crash_xform (rep bxp ixp flist ilist frees mscache) =p=> 
+  Lemma xform_rep : forall bxp ixp flist ilist frees allocc mscache,
+    crash_xform (rep bxp ixp flist ilist frees allocc mscache) =p=> 
       exists flist', [[ flist_crash flist flist' ]] *
-      rep bxp ixp flist' ilist frees mscache.
+      rep bxp ixp flist' ilist frees allocc mscache.
   Proof.
     unfold rep; intros.
     xform_norm.
@@ -2478,11 +2493,11 @@ Module BFILE.
     intuition subst; eauto.
   Qed.
 
-  Lemma xform_rep_file : forall F bxp ixp fs f i ilist frees mscache,
+  Lemma xform_rep_file : forall F bxp ixp fs f i ilist frees allocc mscache,
     (F * i |-> f)%pred (list2nmem fs) ->
-    crash_xform (rep bxp ixp fs ilist frees mscache) =p=> 
+    crash_xform (rep bxp ixp fs ilist frees allocc mscache) =p=> 
       exists fs' f',  [[ flist_crash fs fs' ]] * [[ file_crash f f' ]] *
-      rep bxp ixp fs' ilist frees mscache *
+      rep bxp ixp fs' ilist frees allocc mscache *
       [[ (arrayN_ex (@ptsto _ addr_eq_dec _) fs' i * i |-> f')%pred (list2nmem fs') ]].
   Proof.
     unfold rep; intros.
@@ -2508,12 +2523,12 @@ Module BFILE.
     Unshelve. all: eauto.
   Qed.
 
- Lemma xform_rep_file_pred : forall (F Fd : pred) bxp ixp fs f i ilist frees mscache,
+ Lemma xform_rep_file_pred : forall (F Fd : pred) bxp ixp fs f i ilist frees allocc mscache,
     (F * i |-> f)%pred (list2nmem fs) ->
     (Fd (list2nmem (BFData f))) ->
-    crash_xform (rep bxp ixp fs ilist frees mscache) =p=>
+    crash_xform (rep bxp ixp fs ilist frees allocc mscache) =p=>
       exists fs' f',  [[ flist_crash fs fs' ]] * [[ file_crash f f' ]] *
-      rep bxp ixp fs' ilist frees mscache *
+      rep bxp ixp fs' ilist frees allocc mscache *
       [[ (arrayN_ex (@ptsto _ addr_eq_dec _) fs' i * i |-> f')%pred (list2nmem fs') ]] *
       [[ (crash_xform Fd)%pred (list2nmem (BFData f')) ]].
   Proof.
@@ -2525,12 +2540,12 @@ Module BFILE.
     eapply list2nmem_crash_xform; eauto.
   Qed.
 
-  Lemma xform_rep_off : forall Fm Fd bxp ixp ino off f fs vs ilist frees mscache,
+  Lemma xform_rep_off : forall Fm Fd bxp ixp ino off f fs vs ilist frees allocc mscache,
     (Fm * ino |-> f)%pred (list2nmem fs) ->
     (Fd * off |-> vs)%pred (list2nmem (BFData f)) ->
-    crash_xform (rep bxp ixp fs ilist frees mscache) =p=> 
+    crash_xform (rep bxp ixp fs ilist frees allocc mscache) =p=> 
       exists fs' f' v, [[ flist_crash fs fs' ]] * [[ file_crash f f' ]] *
-      rep bxp ixp fs' ilist frees mscache * [[ In v (vsmerge vs) ]] *
+      rep bxp ixp fs' ilist frees allocc mscache * [[ In v (vsmerge vs) ]] *
       [[ (arrayN_ex (@ptsto _ addr_eq_dec _) fs' ino * ino |-> f')%pred (list2nmem fs') ]] *
       [[ (crash_xform Fd * off |=> v)%pred (list2nmem (BFData f')) ]].
   Proof.
